# Deriving and simplifying $\frac{d}{dm}(\text{MSE})$ and $\frac{d}{db}(\text{MSE})$


We already know that,
<p align = 'center'>$\text{MSE} = \frac{1}{n} \sum_{i=1}^{n} (y_{\text{actual}_i} - y_{\text{predicted}_i})^2 $</p>
Let's denote MSE as E for simplicity:<br>

<p align='center'>$E = \frac{1}{n}\sum_{i=1}^{n}(y_{\text{actual}_i} - y_{\text{predicted}_i})^2$</p>
Now, differentiate E with respect to m:<br>
<p align = 'center'>$\frac{dE}{dm} = \frac{d}{dm} \left( \frac{1}{n} \sum_{i=1}^{n} (y_{\text{actual}_i} - y_{\text{predicted}_i})^2 \right)$</p>
<p>Since $\frac{1}{n}$ is a constant with respect to m, it comes out of the derivative:</p>
<p align='center'>$\frac{dE}{dm} = \frac{1}{n} \cdot \frac{d}{dm} \left( \sum_{i=1}^{n} (y_{\text{actual}_i} - y_{\text{predicted}_i})^2 \right)$</p>
<p>Now, differentiate $(y_{\text{actual}_i} - y_{\text{predicted}_i})^2$ with respect to m:</p>
<p align='center'>$\frac{d}{dm} \left( (y_{\text{actual}_i} - y_{\text{predicted}_i})^2 \right) = 2(y_{\text{actual}_i} - y_{\text{predicted}_i}) \cdot \frac{d}{dm} (y_{\text{actual}_i} - y_{\text{predicted}_i})$</p>
<p>But, the interesting thing is that we already know the value <b>y<sub>actual</sub></b>. So, this is a constant. Isn't it?</p>
<p>So, the final derivation ends with-</p>
<p align='center'>$\frac{d}{dm} \left( (y_{\text{actual}_i} - y_{\text{predicted}_i})^2 \right) = 2(y_{\text{actual}_i} - y_{\text{predicted}_i}) \cdot \frac{d}{dm} (- y_{\text{predicted}_i})$</p>
More simply,
<p align='center'>$\frac{d}{dm} \left( (y_{\text{actual}_i} - y_{\text{predicted}_i})^2 \right) = -2(y_{\text{actual}_i} - y_{\text{predicted}_i}) \cdot \frac{d}{dm} (y_{\text{predicted}_i})$</p>
We know what <b><i>y<sub>predicted</sub></i></b> mean.
<p align='center'>$y_{\text{predicted}_i} = mx_i + b$</p>
