# Go with example
Can you remember, what was our given data?
<br>
> <p align = 'center'><b>x = [1, 2, 3, 4, 5, 6]<br>y<sub>actual</sub> = [1, 4, 9, 16, 25, 36]<br>and<br>m = b = 0</b></p> 

<p>Now, for simplicity, let's start with $x_1$ and $y_{\text{actual}_1}$ <br>So, our initial prediction is $y_{\text{predicted}_1} = m_{\text{old}}x_1 + b_{\text{old}}$</p>
<p>So, $y_{\text{predicted}_1} = 0$</p>
<p>Now, we have to update the values of m and b. Before that, we need to calculate the MSE</p>
<p align='center'>$MSE = (y_{\text{actual}_1} - y_{\text{predicted}_1})^2$ <br> $=(1 - 0)^2$ <br> $= 1$</p>
Now, we can update the values of m and b,<br>
<p>First of all, we have to calculate $\frac{d}{dm}MSE$ and $\frac{d}{db}MSE$</p>
<p align='center'>$\frac{d}{dm}MSE = -2(y_{\text{actual}_1} - y_{\text{predicted}_1})\cdot x_1$ <br>
$=-2(1 - 0)\cdot3$<br>$=-6$</p>
Similarly,
<p align='center'>$\frac{d}{db}MSE = -2$
<p>Now, we have to calculate $m_{\text{new}}$ and $b_{\text{new}}$ as follows-</p>
<p align='center'>$m_{\text{new}} = m_{\text{old}} - α\frac{d}{dm}MSE$ [α is just a learning rate here and let α = 1] <br>
$m_{\text{new}} = 0 - 1\cdot(-6)$<br>$m_{\text{new}} = 6$<br>$b_{\text{new}} = b_{\text{old}} - α\frac{d}{db}MSE$<br>$b_{\text{new}} = 2$</p>
<p>This is how we will update the values of $b_{\text{new}}$ and $m_{\text{new}}$ continuously until the last index of our dataset. Finally, we will reach the final values of them. According to the final values of $m$ and $b$, we can calculate or measure the target value ($y_{\text{predicted}}$) for any new data input value ($x$).</p>
